case_study/RiscvPmpBoundedInts/IrisInstance.v
@@ -75,11 +75,19 @@ Module RiscvPmpIrisInstance <:
       | _ => False
       end.
 
+    Definition addr_inc (x : bv 32) (n : nat) : bv 32 :=
+      bv.add x (bv.of_nat n).
+
+    Definition get_byte {n} (offset : Z) (bits : bv n) : Byte :=
+      bv.of_Z (Z.shiftr (bv.unsigned bits) (offset * 8)).
+
+    (* TODO: change back to words instead of bytes... might be an easier first version
+             and most likely still conventient in the future *)
   Definition femto_inv_ns : ns.namespace := (ns.ndot ns.nroot "ptsto_readonly").
-    Definition interp_ptsto (addr : Addr) (w : Word) : iProp Σ :=
-      mapsto addr (DfracOwn 1) w.
-    Definition interp_ptsto_readonly (addr : Addr) (w : Word) : iProp Σ :=
-      inv femto_inv_ns (interp_ptsto addr w).
+    Definition interp_ptsto (addr : Addr) (b : Byte) : iProp Σ :=
+      mapsto addr (DfracOwn 1) b.
+    Definition interp_ptsto_readonly (addr : Addr) (b : Byte) : iProp Σ :=
+      inv femto_inv_ns (interp_ptsto addr b).
     Definition ptstoSth : Addr -> iProp Σ := fun a => (∃ w, interp_ptsto a w)%I.
     Definition ptstoSthL : list Addr -> iProp Σ :=
       fun addrs => ([∗ list] k↦a ∈ addrs, ptstoSth a)%I.
@@ -93,8 +101,13 @@ Module RiscvPmpIrisInstance <:
     Definition interp_pmp_addr_access_without (addr : Addr) (addrs : list Addr) (entries : list PmpEntryCfg) (m : Privilege) : iProp Σ :=
       (ptstoSth addr -∗ interp_pmp_addr_access addrs entries m)%I.
 
+    Definition interp_ptstomem {width : nat} (addr : Addr) (bytes : bv (width * byte)) : iProp Σ :=
+      [∗ list] offset ∈ (seq 0 width),
+        interp_ptsto (bv.of_Z (bv.unsigned addr + Z.of_nat offset)) (get_byte offset bytes).
+
+    (* TODO: introduce constant for nr of word bytes (replace 4) *)
     Definition interp_ptsto_instr (addr : Addr) (instr : AST) : iProp Σ :=
-      (∃ v, interp_ptsto addr v ∗ ⌜ pure_decode v = inr instr ⌝)%I.
+      (∃ v, @interp_ptstomem 4 addr v ∗ ⌜ pure_decode v = inr instr ⌝)%I.
 
   End WithSailGS.
 
@@ -111,7 +124,7 @@ Module RiscvPmpIrisInstance <:
     | ptsto                    | [ addr; w ]          => interp_ptsto addr w
     | ptsto_readonly           | [ addr; w ]          => interp_ptsto_readonly addr w
     | encodes_instr            | [ code; instr ]      => ⌜ pure_decode code = inr instr ⌝%I
-    | ptstomem                | _                    => True%I
+    | ptstomem _               | [ addr; bs]       => interp_ptstomem addr bs
     | ptstoinstr              | [ addr; instr ]      => interp_ptsto_instr addr instr.
 
     Ltac destruct_pmp_entries :=
